define optimized arrcp

src/arrcp_mcl.lean
@@ -3,15 +3,36 @@ import parlang
 open mcl
 open mcl.mclk
 
+
 namespace arrcp_mcl
 
-def sig : signature
-| _ := { scope := scope.global, type := type.int }
+-- open classical
+-- local attribute [instance] prop_decidable
+-- instance a : decidable_eq string := sorry
+
+#check ([5] : vector _ _)
+
+
+def sig : signature --:= λ n, if n = "i" then { scope := scope.tlocal, type := ⟨_, [1], type.int⟩ } else { scope := scope.global, type := ⟨_, [100], type.int⟩ }
+| "i" := { scope := scope.tlocal, type := ⟨_, [1], type.int⟩ }
+| "tid" := { scope := scope.tlocal, type := ⟨_, [1], type.int⟩ }
+| _ := { scope := scope.global, type := ⟨_, [100], type.int⟩ }
+
+lemma i_is_tlocal : is_tlocal (sig "i") := by apply eq.refl
+lemma a_is_global : is_global (sig "a") := by apply eq.refl
+lemma tid_is_tlocal : is_tlocal (sig "tid") := by apply eq.refl
 
 def arrcp₁ : mclp sig := mclp.intro (λ m, 10) (mclk.global_assign "b" (expression.const_int 7 (by refl)))
 
-def arrcp₂ : mclp sig := mclp.intro (λ m, 10) (mclk.global_assign "c" (expression.const_int 9 (by refl)))
+def read_i := (expression.tlocal_var "i" (λ_, 1) (show type_of (sig "i") = type.int, by apply eq.refl) (by refl) i_is_tlocal)
+def read_tid := (expression.tlocal_var "tid" (λ_, 1) (show type_of (sig "tid") = type.int, by apply eq.refl) (show (sig "tid").type.dim = 1, by apply eq.refl) tid_is_tlocal)
 
+def arrcp₂ : mclp sig := mclp.intro (λ m, 10) (mclk.for "i" (by refl) read_tid (read_i < 100) (mclk.tlocal_assign "i" [1] (show ((sig "i").type).dim = vector.length [1], by refl) (read_i + read_tid)) (
+    mclk.global_assign "b" [read_i] (by refl) (expression.global_var "a" (λ_, read_i) (show type_of (sig "a") = type.int, by refl) (by refl) a_is_global)
+))
+
+#eval mclp_to_program arrcp₂
+#reduce mclp_to_program arrcp₂
 
 example (c) : mclp_to_program arrcp₁ = c := begin
     rw arrcp₁,
